Std/Data/AssocList/WF.lean
@@ -1,0 +1,26 @@
+/-
+Copyright (c) 2024 Lean FRO, LLC. All rights reserved.
+Released under Apache 2.0 license as described in the file LICENSE.
+Authors: Markus Himmel
+-/
+import Std.Classes.BEq
+import Std.Data.AssocList
+
+namespace Std.AssocList
+
+/-- The well-formedness predicate for associative lists says that the keys are pairwise distinct. -/
+structure WF [BEq α] (l : AssocList α β) : Prop where
+  /-- The keys of a well-formed associative list are pairwise distinct. -/
+  distinct [PartialEquivBEq α] : l.keys.Pairwise fun a b => (a == b) = false
+
+@[simp]
+theorem WF.nil [BEq α] : (.nil : AssocList α β).WF :=
+  ⟨by simp⟩
+
+theorem WF.cons [BEq α] {l : AssocList α β} {k : α} {v : β} (h : l.contains k = false) :
+    (l.cons k v).WF := sorry
+
+theorem WF.replace [BEq α] {l : AssocList α β} {k : α} {v : β} :
+    (l.replace k v).WF := sorry
+
+end Std.AssocList
